src/riscv/Spec/Primitives.v
@@ -33,10 +33,10 @@ Section Primitives.
     is_initial_register_value: word -> Prop;
 
     (* tells what happens if an n-byte read at a non-memory address is performed *)
-    nonmem_load: forall (n: nat), SourceType -> word -> M (HList.tuple byte n);
+    nonmem_load : forall (n: nat), SourceType -> word -> RiscvMachine -> (HList.tuple byte n -> RiscvMachine -> Prop) -> Prop;
 
     (* tells what happens if an n-byte write at a non-memory address is performed *)
-    nonmem_store: forall (n: nat), SourceType -> word -> HList.tuple byte n -> M unit;
+    nonmem_store: forall (n: nat), SourceType -> word -> HList.tuple byte n -> RiscvMachine -> (RiscvMachine -> Prop) -> Prop;
   }.
 
   Class mcomp_sat_spec{Machine: Type}(p: PrimitivesParams Machine): Prop := {
@@ -97,7 +97,7 @@ Section Primitives.
       ((exists v, mem_load initialL.(getMem) addr = Some v /\
                   post v initialL) \/
        (mem_load initialL.(getMem) addr = None /\
-        mcomp_sat (nonmem_load n kind addr) initialL post)) <->
+        nonmem_load n kind addr initialL post)) <->
       mcomp_sat (riscv_load kind addr) initialL post.
 
   Definition clear_lowest_two_bits(w: word): word :=
@@ -122,7 +122,7 @@ Section Primitives.
                   post tt (withXAddrs (invalidateWrittenXAddrs n addr initialL.(getXAddrs))
                           (withMem m' initialL))) \/
       (mem_store initialL.(getMem) addr v = None /\
-       mcomp_sat (nonmem_store n kind addr v) initialL post) <->
+       nonmem_store n kind addr v initialL (post tt)) <->
       mcomp_sat (riscv_store kind addr v) initialL post.
 
   (* primitives_params is a paramater rather than a field because Primitives lives in Prop and
@@ -173,4 +173,4 @@ Section Primitives.
 
 End Primitives.
 
-Arguments PrimitivesParams {_} M Machine.
+Arguments PrimitivesParams {_ _ _} M Machine.
